FSM/Util.thy
@@ -910,29 +910,47 @@ lemma subset_list_set : "subset_list xs ys = ((set xs) \<subseteq> (set ys))"
   by (simp add: Ball_set subset_code(1)) 
 
 
+
 subsection \<open>Calculating Distinct Non-Reflexive Pairs over List Elements\<close> 
 
-fun non_refl_dist_pairs :: "'a list \<Rightarrow> ('a \<times> 'a) list" where
-  "non_refl_dist_pairs [] = []" |
-  "non_refl_dist_pairs (x#xs) = (map (\<lambda> y. (x,y)) xs) @ non_refl_dist_pairs xs"
+(* Could be used to calculate tuples ((q1,q2),A), where A is a separator for q1 q2, such that
+   ((q2,q1),_) is skipped *)
 
-value "non_refl_dist_pairs [1,2,3::nat]"
+fun non_refl_dist_pairs' :: "'a list \<Rightarrow> ('a \<times> 'a) list" where
+  "non_refl_dist_pairs' [] = []" |
+  "non_refl_dist_pairs' (x#xs) = (map (\<lambda> y. (x,y)) xs) @ non_refl_dist_pairs' xs"
+
+fun non_refl_dist_pairs :: "'a list \<Rightarrow> ('a \<times> 'a) list" where
+  "non_refl_dist_pairs xs = non_refl_dist_pairs' (remdups xs)"
+
+value "non_refl_dist_pairs' [1,2,3::nat]"
+value "non_refl_dist_pairs' [1,2,1,3::nat]"
+value "non_refl_dist_pairs [1,2,1,3::nat]"
 
 lemma non_refl_dist_pairs_subset : "set (non_refl_dist_pairs xs) \<subseteq> (set xs) \<times> (set xs)"
   by (induction xs; auto)
 
-lemma non_refl_dist_pairs_elems_distinct:
+lemma non_refl_dist_pairs'_elems_distinct:
   assumes "distinct xs"
-  and     "(x,y) \<in> set (non_refl_dist_pairs xs)"
+  and     "(x,y) \<in> set (non_refl_dist_pairs' xs)"
 shows "x \<in> set xs" 
 and   "y \<in> set xs"
 and   "x \<noteq> y"
 proof -
   show "x \<in> set xs" and "y \<in> set xs"
-    using non_refl_dist_pairs_subset assms(2) by auto
+    using non_refl_dist_pairs_subset assms(2) by (induction xs; auto)+
   show "x \<noteq> y"
     using assms by (induction xs; auto)
 qed
+
+lemma non_refl_dist_pairs_elems_distinct:
+  assumes "(x,y) \<in> set (non_refl_dist_pairs xs)"
+shows "x \<in> set xs" 
+and   "y \<in> set xs"
+and   "x \<noteq> y"
+  using non_refl_dist_pairs'_elems_distinct assms
+  unfolding non_refl_dist_pairs.simps by fastforce+
+
 
 lemma non_refl_dist_pairs_elems :
   assumes "x \<in> set xs"
@@ -943,15 +961,57 @@ shows "(x,y) \<in> set (non_refl_dist_pairs xs) \<or> (y,x) \<in> set (non_refl_
 
 
 
-lemma non_refl_dist_pairs_elems :
+lemma non_refl_dist_pairs'_elems_non_refl :
   assumes "distinct xs"
-  and     "(x,y) \<in> set (non_refl_dist_pairs xs)"
-shows "(y,x) \<notin> set (non_refl_dist_pairs xs)"
-  using assms non_refl_dist_pairs_elems_distinct[OF assms] 
+  and     "(x,y) \<in> set (non_refl_dist_pairs' xs)"
+shows "(y,x) \<notin> set (non_refl_dist_pairs' xs)"
+  using assms  
+proof (induction xs arbitrary: x y)
+  case Nil
+  then show ?case by auto
+next
+  case (Cons z zs)
+  then have "distinct zs" by auto
 
-(* TODO*)
+  have "x \<noteq> y"
+    using non_refl_dist_pairs'_elems_distinct[OF Cons.prems] by simp
 
-end (*
+  consider (a) "(x,y) \<in> set (map (Pair z) zs)" |
+           (b) "(x,y) \<in> set (non_refl_dist_pairs' zs)"
+    using \<open>(x,y) \<in> set (non_refl_dist_pairs' (z#zs))\<close> unfolding non_refl_dist_pairs'.simps by auto
+  then show ?case proof cases
+    case a
+    then have "x = z" by auto
+    then have "(y,x) \<notin> set (map (Pair z) zs)"
+      using \<open>x \<noteq> y\<close> by auto
+    moreover have "x \<notin> set zs"
+      using \<open>x = z\<close> \<open>distinct (z#zs)\<close> by auto
+    ultimately show ?thesis 
+      using \<open>distinct zs\<close> non_refl_dist_pairs'_elems_distinct(2) by fastforce
+  next
+    case b
+    then have "x \<noteq> z" and "y \<noteq> z"
+      using Cons.prems unfolding non_refl_dist_pairs'.simps 
+      by (meson distinct.simps(2) non_refl_dist_pairs'_elems_distinct(1,2))+
+    
+    then show ?thesis 
+      using Cons.IH[OF \<open>distinct zs\<close> b] by auto
+  qed
+qed
+
+
+lemma non_refl_dist_pairs_elems_non_refl :
+  assumes "(x,y) \<in> set (non_refl_dist_pairs xs)"
+  shows "(y,x) \<notin> set (non_refl_dist_pairs xs)"
+  using assms by (simp add: non_refl_dist_pairs'_elems_non_refl)
+
+
+lemma non_refl_dist_pairs_set_iff :
+  "(x,y) \<in> set (non_refl_dist_pairs xs) \<longleftrightarrow> (x \<noteq> y \<and> x \<in> set xs \<and> y \<in> set xs \<and> (y,x) \<notin> set (non_refl_dist_pairs xs))"
+  using non_refl_dist_pairs_elems_non_refl[of x y xs] 
+        non_refl_dist_pairs_elems[of x xs y] 
+        non_refl_dist_pairs_elems_distinct[of x y xs] by blast 
+
 
 
 subsection \<open>Other Lemmata\<close>
